add bit and phase flips for nine qubit code

examples/error-correction/NineQubitCode.v
@@ -1,6 +1,7 @@
 Require Export SQIR.UnitaryOps.
 
 Require Import Common.
+Import Common.
 
 Module NineQubitCode.
 
@@ -8,27 +9,30 @@ Local Open Scope ucom.
 Local Open Scope nat_scope.
 
 Notation dim := 9%nat.
+Notation block_dim := 3%nat.
+
+Local Opaque CCX.
 
 (** 
   Blocks
  *)
 
 Inductive up_to_three :=
-  | Zero 
+  | Zer0 
   | One
   | Two.
 
 Definition t_to_nat (t : up_to_three) : nat :=
   match t with
-  | Zero => 0
+  | Zer0 => 0
   | One  => 1
   | Two  => 2
   end.
 
 Definition t_eq (t₁ t₂ : up_to_three) : bool :=
   match t₁, t₂ with
-  | Zero, Zero
-| One, One
+  | Zer0, Zer0
+  | One, One
   | Two, Two => true
   | _, _ => false
   end.
@@ -38,7 +42,7 @@ Coercion t_to_nat : up_to_three >-> nat.
 Definition t_of_nat (n : nat) (h : n < 3) : up_to_three.
 Proof.
   destruct n as [| [| [| n']]].
-  - exact Zero.
+  - exact Zer0.
   - exact One.
   - exact Two.
   - lia.
@@ -53,62 +57,102 @@ Definition block_offset := up_to_three.
 Definition block_to_qubit (n : block_no) (off : block_offset) : nat :=
   n * 3 + off.
 
-Compute block_to_qubit (t_of_nat 2 ltac:(lia)) (t_of_nat 2 ltac:(lia)).
+Ltac compute_vec :=
+    simpl uc_eval;
+    repeat rewrite Mmult_assoc; restore_dims;
+    repeat Common.f_to_vec_simpl_light;
+    simpl;
+    replace (0 * PI)%R with 0%R by lra;
+    replace (1 * PI)%R with PI by lra;
+    autorewrite with Cexp_db;
+    repeat rewrite Mscale_1_l;
+    restore_dims;
+    autorewrite with ket_db.
+
+Ltac correct_inPar well_typed :=
+  try
+  (replace (@uc_eval 9) with (@uc_eval (3 + 6)) by easy;
+   rewrite inPar_correct by well_typed);
+  try 
+  (replace (@uc_eval 6) with (@uc_eval (3 + 3)) by easy;
+   rewrite inPar_correct by well_typed);
+  restore_dims.
 
 (**
   Encoding
  *)
 
-Definition encode_block (n : block_no) : base_ucom dim :=
-  let q0 := n * 3 in
-  let q1 := q0 + 1 in
-  let q2 := q0 + 2 in
-  H q0;
-  CNOT q0 q1;
-  CNOT q0 q2.
+Definition encode_block : base_ucom block_dim :=
+  H 0;
+  CNOT 0 1;
+  CNOT 0 2.
+
+Theorem encode_block_zero :
+  uc_eval encode_block × ∣0,0,0⟩
+  = / √ 2 .* (∣ 0, 0, 0 ⟩ .+ ∣ 1, 1, 1 ⟩).
+Proof.
+  rewrite Common.zero_3_f_to_vec.
+  compute_vec.
+  reflexivity.
+Qed.
+
+
+Theorem encode_block_one :
+  uc_eval encode_block × ∣1,0,0⟩
+  = / √ 2 .* (∣ 0, 0, 0 ⟩ .+ (-1)%R .* ∣ 1, 1, 1 ⟩).
+Proof.
+  replace (∣1,0,0⟩) with (f_to_vec 3 (fun n => n =? 0)) by lma'.
+  compute_vec.
+  reflexivity.
+Qed.
+
+Theorem encode_block_well_typed :
+  uc_well_typed encode_block.
+Proof.
+  unfold encode_block.
+  auto.
+  constructor.
+  - constructor.
+    + apply uc_well_typed_H; lia.
+    + apply uc_well_typed_CNOT; lia.
+  - apply uc_well_typed_CNOT; lia.
+Qed.
 
 Definition encode : base_ucom dim :=
   CNOT 0 3; CNOT 0 6;
-  encode_block (t_of_nat 0 ltac:(lia));
-  encode_block (t_of_nat 1 ltac:(lia));
-  encode_block (t_of_nat 2 ltac:(lia)).
+  inPar encode_block (inPar encode_block encode_block).
 
 Notation encoded α β := (
-    /C2 .* (/√ 2 .* (α .* (3 ⨂ (∣0,0,0⟩ .+            ∣1,1,1⟩))))
- .+ /C2 .* (/√ 2 .* (β .* (3 ⨂ (∣0,0,0⟩ .+  (-1)%R .* ∣1,1,1⟩))))
+    α .* (/C2 .* (/√ 2 .* (3 ⨂ (∣0,0,0⟩ .+            ∣1,1,1⟩))))
+ .+ β .* (/C2 .* (/√ 2 .* (3 ⨂ (∣0,0,0⟩ .+  (-1)%R .* ∣1,1,1⟩))))
 ).
 
-Ltac f_to_vec_simpl_light :=
-  first
-  [ rewrite f_to_vec_H
-  | rewrite f_to_vec_CCX
-  | rewrite f_to_vec_CNOT
-  ];
-  try lia;
-  simpl update;
-  do 2 (
-    repeat rewrite Mmult_plus_distr_l;
-    repeat rewrite Mscale_mult_dist_r
-  ).
 
-Ltac pull_scalars :=
-  repeat rewrite <- Mscale_plus_distr_r;
-  repeat rewrite kron_plus_distr_r;
-  repeat rewrite kron_plus_distr_l;
-  repeat rewrite Mplus_assoc.
+Ltac reorder_scalars :=
+  repeat rewrite Mscale_assoc;
+  repeat rewrite Cmult_comm with (x := ((-1)%R : C));
+  repeat rewrite <- Mscale_assoc with (y := ((-1)%R : C));
+  repeat rewrite <- Mscale_plus_distr_r.
+
+Ltac normalize_kron_notation :=
+  repeat rewrite <- kron_assoc by auto 8 with wf_db;
+  try easy.
+
+Lemma inv_sqrt2_cubed : (/ √ 2 * / √ 2 * / √ 2)%C = (/ C2 * /√ 2)%C.
+Proof.
+  now rewrite Cinv_sqrt2_sqrt.
+Qed.
 
 Theorem encode_correct : forall (α β : C),
    (@uc_eval dim encode) × ((α .* ∣0⟩ .+ β .* ∣1⟩) ⊗ 8 ⨂ ∣0⟩)
    = encoded α β.
 Proof.
   intros.
+  Local Opaque inPar.
   simpl. Msimpl_light.
-
   replace (∣0⟩) with (f_to_vec 1 (fun _ => false)) by lma'.
   replace (∣1⟩) with (f_to_vec 1 (fun _ => true)) by lma'.
   restore_dims.
-  rewrite Common.zero_9_f_to_vec.
-  rewrite Common.nine_9_f_to_vec.
 
   repeat rewrite Mmult_assoc.
   rewrite kron_plus_distr_r.
@@ -118,50 +162,26 @@ Proof.
   restore_dims.
   repeat rewrite kron_assoc by auto 10 with wf_db.
   repeat (rewrite f_to_vec_merge; restore_dims).
-  
-  repeat f_to_vec_simpl_light.
+
+  repeat Common.f_to_vec_simpl_light.
   simpl. Msimpl_light.
-
-  replace (0 * PI)%R with 0%R by lra.
-  replace (1 * PI)%R with PI by lra.
-  autorewrite with Cexp_db.
-  group_radicals.
-  repeat rewrite Mscale_1_l.
-
-  pull_scalars.
-  f_equal.
-  - repeat rewrite Mscale_assoc.
-    replace (α * / √ 2 * / √ 2 * / √ 2)%C with (/√ 2 * / C2 * α)%C.
-    2: {
-      (* why does lca not work here? *)
-      rewrite Cmult_comm.
-      do 2 rewrite <- Cmult_assoc.
-      f_equal. f_equal.
-      symmetry. apply Cinv_sqrt2_sqrt.
-    }
-    repeat (rewrite <- kron_assoc by auto 10 with wf_db; restore_dims).
-    reflexivity.
-  - do 2 (
-      repeat rewrite Mscale_assoc;
-      repeat rewrite (Cmult_comm (-1)%R _);
-      repeat rewrite <- (Mscale_assoc _ _ _ (-1)%R _);
-      repeat rewrite <- Mscale_plus_distr_r
-    ).
-    repeat rewrite Mscale_assoc.
-    replace (β * / √ 2 * / √ 2 * / √ 2)%C with (/ √ 2 * / C2 * β)%C.
-    2: {
-      (* why does lca not work here? *)
-      rewrite Cmult_comm.
-      do 2 rewrite <- Cmult_assoc.
-      f_equal. f_equal.
-      symmetry. apply Cinv_sqrt2_sqrt.
-    }
-    f_equal.
-    repeat rewrite Mscale_plus_distr_r.
-    distribute_scale.
-    repeat (rewrite <- kron_assoc by auto 10 with wf_db; restore_dims).
-    repeat rewrite Mplus_assoc.
-    reflexivity.
+  restore_dims.
+  correct_inPar ltac:(apply encode_block_well_typed).
+  replace (∣0, 0, 0, 0, 0, 0, 0, 0, 0⟩) with (∣0, 0, 0⟩ ⊗ ∣0, 0, 0, 0, 0, 0⟩) by normalize_kron_notation.
+  replace (∣0, 0, 0, 0, 0, 0⟩) with (∣0, 0, 0⟩ ⊗ ∣0, 0, 0⟩) by normalize_kron_notation.
+  replace (∣1, 0, 0, 1, 0, 0, 1, 0, 0⟩) with (∣1, 0, 0⟩ ⊗ ∣1, 0, 0, 1, 0, 0⟩) by normalize_kron_notation.
+  replace (∣1, 0, 0, 1, 0, 0⟩) with (∣1, 0, 0⟩ ⊗ ∣1, 0, 0⟩) by normalize_kron_notation.
+  restore_dims.
+  do 4 rewrite kron_mixed_product.
+  rewrite encode_block_zero, encode_block_one.
+  repeat rewrite Mscale_kron_dist_l.
+  repeat rewrite Mscale_kron_dist_r.
+  normalize_kron_notation.
+  repeat rewrite <- Cmult_assoc.
+  repeat rewrite <- inv_sqrt2_cubed.
+  repeat rewrite Cmult_assoc.
+  repeat rewrite Mscale_assoc.
+  reflexivity.
 Qed.
 
 
@@ -173,33 +193,49 @@ Inductive phase_flip_error (n : block_no) : Set :=
   | OnePhaseFlip (off : block_offset)
   | MorePhaseFlip (e : phase_flip_error n) (off : block_offset).
 
+Fixpoint phase_flip_odd_parity {n : block_no} (e : phase_flip_error n) : bool :=
+  match e with
+  | OnePhaseFlip _ _ => true
+  | MorePhaseFlip _ e _ => negb (phase_flip_odd_parity e)
+  end.
+
 Inductive bit_flip_error : Set :=
   | OneBitFlip (n : block_no) (off : block_offset)
-  | TwoBitFlip (n₁ n₂ : block_no) (h : n₁ <> n₂) (off₁ off₂ : block_offset)
+  | TwoBitFlip (safe_n : block_no) (off₁ off₂ : block_offset)
   | ThreeBitFlip (off₁ off₂ off₃ : block_offset).
 
 Inductive error : Set :=
   | NoError
   | PhaseFlipError {n} (e : phase_flip_error n)
   | BitFlipError (e : bit_flip_error)
-  | PhaseBitErrors {phase_n} (e₁ : phase_flip_error phase_n) (e₂ : bit_flip_error)
-  | BitPhaseErrors (e₁ : bit_flip_error) {phase_n} (e₂ : phase_flip_error phase_n).
+  | PhaseBitErrors {phase_n} (e₁ : phase_flip_error phase_n) (e₂ : bit_flip_error).
+
+Definition apply_to_block (n : block_no) (uc : base_ucom block_dim) :=
+  match n with
+  | Zer0 => inPar uc   (inPar SKIP SKIP)
+  | One  => inPar SKIP (inPar uc SKIP)
+  | Two  => inPar SKIP (inPar SKIP uc)
+  end.
 
 Fixpoint apply_phase_flip_error {n} (e : phase_flip_error n) : base_ucom dim :=
   match e with
-  | OnePhaseFlip _ off => SQIR.Z off
-  | MorePhaseFlip _ e off => SQIR.Z off; apply_phase_flip_error e
+  | OnePhaseFlip _ off => apply_to_block n (SQIR.Z off)
+  | MorePhaseFlip _ e off => 
+      apply_to_block n (SQIR.Z off);
+      apply_phase_flip_error e
   end.
 
-Definition apply_bit_flip_error (e : bit_flip_error) : base_ucom dim :=
+Definition apply_bit_flip_error (e : bit_flip_error) : base_ucom (block_dim + (block_dim + block_dim)) :=
   match e with
-  | OneBitFlip n off => X (block_to_qubit n off)
-  | TwoBitFlip n₁ n₂ _ off₁ off₂ => (X (block_to_qubit n₁ off₁)); (X (block_to_qubit n₂ off₂))
+  | OneBitFlip n off => apply_to_block n (X off)
+  | TwoBitFlip safe_n off₁ off₂ =>
+      match safe_n with
+      | Zer0 => inPar SKIP (inPar (X off₁) (X off₂))
+      | One => inPar (X off₁) (inPar SKIP (X off₂))
+      | Two => inPar (X off₁) (inPar (X off₂) SKIP)
+      end
   | ThreeBitFlip off₁ off₂ off₃ => (
-    let q1 := block_to_qubit (t_of_nat 0 ltac:(lia)) off₁ in
-    let q2 := block_to_qubit (t_of_nat 1 ltac:(lia)) off₂ in
-    let q3 := block_to_qubit (t_of_nat 2 ltac:(lia)) off₃ in
-    X q1; X q2; X q3
+    inPar (X off₁) (inPar (X off₂) (X off₃))
   )
   end.
 
@@ -209,7 +245,6 @@ Definition apply_error (e : error) : base_ucom dim :=
   | PhaseFlipError    e  => apply_phase_flip_error e
   | BitFlipError      e  => apply_bit_flip_error e
   | PhaseBitErrors e₁ e₂ => apply_phase_flip_error e₁; apply_bit_flip_error e₂
-  | BitPhaseErrors e₁ e₂ => apply_bit_flip_error e₁; apply_phase_flip_error e₂
   end.
 
 Fixpoint list_to_map (l : list nat) : nat -> bool :=
@@ -224,37 +259,33 @@ Fixpoint ancillae_for_phase_flip {n} (e : phase_flip_error n) : list nat :=
   | MorePhaseFlip _ (MorePhaseFlip _ e _) _ => ancillae_for_phase_flip e
   | OnePhaseFlip _ _ => 
       match n with 
-      | Zero => 3 :: [6]
-      | One  => [3]
-      | Two  => [6]
+      | Zer0 => 2 :: [5]
+      | One  => [2]
+      | Two  => [5]
       end
   end.
 
-Definition block_to_syn (b : block_no) (off : block_offset) : list nat :=
+Definition block_to_bit_syn (b : block_no) (off : block_offset) : list nat :=
+  let left_edge := b * 3 in
   match off with
-  | Zero => b + 1 :: [b + 2]
-  | One  => [b + 1]
-  | Two  => [b + 2]
+  | Zer0        => left_edge :: [left_edge + 1]
+  | One         => [left_edge]
+  | Two         => [left_edge + 1]
   end.
 
 Definition ancillae_for_bit_flip (e : bit_flip_error) : list nat :=
   match e with
-| OneBitFlip n off => block_to_syn n off
-  | TwoBitFlip n₁ n₂ h off₁ off₂ => 
-      match n₁ as n₁', n₂ as n₂' return n₁ = n₁' -> n₂ = n₂' -> list nat with
-      | Zero, Zero
-      | One, One
-      | Two, Two => fun h₁ h₂ => ltac:(
-          exfalso;
-          subst;
-          contradiction
-      )
-      | n₁', n₂' => fun _ _ => (block_to_syn n₁' off₁) ++ (block_to_syn n₂' off₂)
-      end eq_refl eq_refl
-  | ThreeBitFlip off₁ off₂ off₃ =>
-      (block_to_syn (t_of_nat 0 ltac:(lia)) off₁) ++
-      (block_to_syn (t_of_nat 1 ltac:(lia)) off₂) ++
-      (block_to_syn (t_of_nat 2 ltac:(lia)) off₃)
+  | OneBitFlip n off => block_to_bit_syn n off
+  | TwoBitFlip safe_n off₁ off₂ => 
+      match safe_n with
+      | Zer0 => (block_to_bit_syn One off₁) ++ (block_to_bit_syn Two off₂)
+      | One => (block_to_bit_syn Zer0 off₁) ++ (block_to_bit_syn Two off₂)
+      | Two => (block_to_bit_syn Zer0 off₁) ++ (block_to_bit_syn One off₂)
+      end
+      | ThreeBitFlip off₁ off₂ off₃ =>
+          (block_to_bit_syn Zer0 off₁) ++
+          (block_to_bit_syn One  off₂) ++
+          (block_to_bit_syn Two  off₃)
   end.
 
 Definition ancillae_for (e : error) : Vector (2 ^ 8) :=
@@ -267,40 +298,109 @@ Definition ancillae_for (e : error) : Vector (2 ^ 8) :=
         ancillae_for_phase_flip e₁ ++
         ancillae_for_bit_flip e₂
       ))
-  | @BitPhaseErrors e₁ phase_n e₂ => 
-      let v := f_to_vec 8 (list_to_map (
-          ancillae_for_bit_flip e₁ ++
-          ancillae_for_phase_flip e₂
-        )) in
-      match e₁ with
-      | OneBitFlip n off => 
-          if t_eq n phase_n
-          then (-1)%R .* v
-          else v
-      | TwoBitFlip n₁ n₂ _ _ _ =>
-          if orb (t_eq n₁ phase_n) (t_eq n₂ phase_n)
-          then (-1)%R .* v
-          else v
-      | ThreeBitFlip _ _ _ => (-1)%R .* v
-      end
   end.
 
-Definition decode_block (n : block_no) : base_ucom dim :=
-  let q0 := n * 3 in
-  let q1 := q0 + 1 in
-  let q2 := q0 + 2 in
-  CNOT q0 q1;
-  CNOT q0 q2;
-  CCX q1 q2 q0;
-  H q0.
+Lemma ancillae_for_two_phases_cancel {n}: 
+  forall (e : phase_flip_error n) (off₁ off₂ : block_offset),
+  ancillae_for (PhaseFlipError (MorePhaseFlip n (MorePhaseFlip n e off₁) off₂))
+  = ancillae_for (PhaseFlipError e).
+Proof.
+  easy.
+Qed.
+
+Definition decode_block : base_ucom block_dim :=
+  CNOT 0 1;
+  CNOT 0 2;
+  CCX 1 2 0;
+  H 0.
+
+Theorem decode_block_well_typed : uc_well_typed decode_block.
+Proof.
+  repeat constructor.
+  Local Transparent CCX.
+  all : unfold CCX.
+  Local Opaque CCX.
+  3 : repeat constructor.
+  all : unfold TDAG.
+  all : try apply uc_well_typed_H; try lia.
+  all : try apply uc_well_typed_CNOT; try lia.
+  all : try apply uc_well_typed_Rz; lia.
+Qed.
+
+
+Lemma decode_block_zero :
+  uc_eval decode_block × ∣0,0,0⟩ = / √ 2 .* (∣0,0,0⟩ .+ ∣1,0,0⟩).
+Proof.
+  rewrite Common.zero_3_f_to_vec.
+  compute_vec.
+  reflexivity.
+Qed.
+
+Lemma decode_block_one :
+  uc_eval decode_block × ∣1,0,0⟩ = / √ 2 .* (∣0,1,1⟩ .+ ∣1,1,1⟩).
+Proof.
+  rewrite Common.one_3_f_to_vec.
+  now compute_vec.
+Qed.
+
+Lemma decode_block_two :
+  uc_eval decode_block × ∣0,1,0⟩ = / √ 2 .* (∣0,1,0⟩ .+ ∣1,1,0⟩).
+Proof.
+  rewrite Common.two_3_f_to_vec.
+  now compute_vec.
+Qed.
+
+Lemma decode_block_three :
+  uc_eval decode_block × ∣1,1,0⟩ = / √ 2 .* (∣0,0,1⟩ .+ (-1)%R .* ∣1,0,1⟩).
+Proof.
+  rewrite Common.three_3_f_to_vec.
+  now compute_vec.
+Qed.
+
+Lemma decode_block_four :
+  uc_eval decode_block × ∣0,0,1⟩ = / √ 2 .* (∣0,0,1⟩ .+ ∣1,0,1⟩).
+Proof.
+  rewrite Common.four_3_f_to_vec.
+  now compute_vec.
+Qed.
+
+Lemma decode_block_five :
+  uc_eval decode_block × ∣1,0,1⟩ = / √ 2 .* (∣0,1,0⟩ .+ (-1)%R .* ∣1,1,0⟩).
+Proof.
+  rewrite Common.five_3_f_to_vec.
+  now compute_vec.
+Qed.
+
+Lemma decode_block_six :
+  uc_eval decode_block × ∣0,1,1⟩ = / √ 2 .* (∣0,1,1⟩ .+ (-1)%R .* ∣1,1,1⟩).
+Proof.
+  rewrite Common.six_3_f_to_vec.
+  now compute_vec.
+Qed.
+
+Lemma decode_block_seven :
+  uc_eval decode_block × ∣1,1,1⟩ = / √ 2 .* (∣0,0,0⟩ .+ (-1)%R .* ∣1,0,0⟩).
+Proof.
+  rewrite Common.seven_3_f_to_vec.
+  now compute_vec.
+Qed.
+
+#[export] Hint Rewrite
+  decode_block_zero
+  decode_block_one
+  decode_block_two
+  decode_block_three
+  decode_block_four
+  decode_block_five
+  decode_block_six
+  decode_block_seven
+  : decode_block_db.
 
 (**
   Decode
  *)
 Definition decode : base_ucom dim := 
-  decode_block (t_of_nat 0 ltac:(lia));
-  decode_block (t_of_nat 1 ltac:(lia));
-  decode_block (t_of_nat 2 ltac:(lia));
+  inPar decode_block (inPar decode_block decode_block);
   CNOT 0 3; CNOT 0 6;
   CCX 6 3 0.
 
@@ -313,206 +413,359 @@ Definition shor (e : error) : base_ucom dim :=
   (* Does not use the regular:
      `encode; apply_error e; recover; decode` 
      (because we do not recover the original encoding).
-     Attempting to do so requires 8 addition
+     Attempting to do so requires 8 additional
      qubits (really classical bits), 2 per block
      for bit flip, and 2 for phase flip.
      This makes the following analysis rougher.
   *)
   decode.
 
-Lemma inv_sqrt2_cubed : (/ √ 2 * / √ 2 * / √ 2)%C = (/ C2 * /√ 2)%C.
+Lemma uc_well_typed_SKIP {d} {h : 0 < d} :
+  @uc_well_typed _ d SKIP.
 Proof.
-  rewrite Cinv_sqrt2_sqrt.
-  easy.
+  unfold SKIP.
+  apply uc_well_typed_ID.
+  assumption.
 Qed.
 
-Ltac compute_vec :=
-    simpl uc_eval;
-    repeat rewrite Mmult_assoc; restore_dims;
-    repeat f_to_vec_simpl_light;
-    simpl;
-    replace (0 * PI)%R with 0%R by lra;
-    replace (1 * PI)%R with PI by lra;
-    autorewrite with Cexp_db;
-    repeat rewrite Mscale_1_l;
-    restore_dims;
-    autorewrite with ket_db.
+Ltac simplify_sums :=
+  match goal with
+    | [ |- context [ (?A .+ ?B)
+                    .+ (?A .+ RtoC (-1)%R .* ?B) ]
+      ] => 
+      replace (A .+ B
+                .+ (A .+ RtoC (-1)%R .* B)) with (C2 .* A) by lma
+    | [ |- context [?A .+ ?B
+                      .+ RtoC (-1)%R .* (?A .+ RtoC (-1)%R .* ?B)]
+      ] =>
+        replace (A .+ B
+                  .+ RtoC (-1)%R .* (A .+ RtoC (-1)%R .* B))
+            with (C2 .* B) by lma
+  end.
 
-Ltac prep_err_compute :=
-  simpl; Msimpl_light; restore_dims;
-  rewrite Common.zero_9_f_to_vec, Common.nine_9_f_to_vec;
-  repeat (rewrite kron_plus_distr_r, kron_plus_distr_l; restore_dims);
-  repeat rewrite kron_plus_distr_r;
-  repeat rewrite Mplus_assoc;
-  repeat (rewrite Mscale_kron_dist_l; restore_dims);
-  repeat rewrite Mscale_kron_dist_r;
-  repeat (rewrite Mscale_kron_dist_l; restore_dims);
+Ltac pull_scalars :=
+  distribute_scale;
+  repeat rewrite Mscale_mult_dist_r;
+  repeat rewrite Mscale_assoc.
+
+Lemma collapse_scalar :
+  (/ C2 * (/ √ 2 * (/ √ 2 * (C2 * (/ √ 2 * (C2 * (/ √ 2 * C2)))))))%C = C1.
+Proof. C_field. Qed.
+
+Ltac distribute_over_blocks :=
+  repeat rewrite kron_1_l by auto 10 with wf_db;
+  repeat rewrite kron_assoc by auto with wf_db;
+  repeat rewrite Mmult_plus_distr_l;
+  repeat rewrite Mscale_mult_dist_r;
+  repeat rewrite Mmult_assoc;
+  restore_dims;
+  repeat rewrite kron_mixed_product;
+  repeat rewrite Mmult_plus_distr_l;
+  normalize_kron_notation;
+  repeat rewrite Mscale_mult_dist_r.
+
+
+Ltac flatten :=
+  rewrite kron_plus_distr_r;
+  rewrite 2 Mscale_kron_dist_l;
+  rewrite ket0_equiv, ket1_equiv;
+  repeat (rewrite <- kron_assoc by auto 9 with wf_db; restore_dims).
+
+Ltac compute_decoding := 
+  repeat rewrite kron_1_l by auto with wf_db;
+  repeat rewrite <- Mmult_assoc;
+  rewrite Mmult_plus_distr_l;
+  repeat rewrite Mscale_mult_dist_r;
+  repeat rewrite Mmult_assoc;
+  correct_inPar ltac:(apply decode_block_well_typed);
+  restore_dims;
+  distribute_over_blocks;
+  restore_dims;
+  
+  autorewrite with decode_block_db;
+
+  restore_dims;
+  reorder_scalars;
+  repeat simplify_sums;
+  pull_scalars;
+  rewrite Common.zero_3_f_to_vec;
+  rewrite Common.one_3_f_to_vec;
+
+  restore_dims;
+  repeat rewrite kron_assoc by auto 10 with wf_db;
   repeat (rewrite f_to_vec_merge; restore_dims);
+  repeat Common.f_to_vec_simpl_light;
+  simpl; Qsimpl;
+  repeat rewrite <- Cmult_assoc;
+  rewrite collapse_scalar;
+  autorewrite with C_db;
 
-  repeat rewrite Mmult_plus_distr_l;
-  repeat rewrite Mscale_mult_dist_r;
+  now flatten.
 
-  repeat rewrite Mmult_plus_distr_l;
-  repeat rewrite Mscale_mult_dist_r;
-  restore_dims.
+Theorem decode_correct :
+  forall (α β : C),
+  (@uc_eval dim decode) × encoded α β
+  = (α .* ∣0⟩ .+ β .* ∣1⟩) ⊗ 8 ⨂ ∣0⟩.
+Proof.
+  intros. simpl uc_eval.
+  Qsimpl. simpl.
+  now compute_decoding.
+Qed.
 
 
-Ltac post_compute_vec :=
-    repeat rewrite Cmult_assoc;
-    rewrite inv_sqrt2_cubed;
-    repeat rewrite <- Mscale_assoc with (y := ((-1)%R : C));
-    repeat rewrite <- Mscale_plus_distr_r;
-    repeat rewrite <- kron_assoc; auto with wf_db;
-
-    repeat rewrite Mplus_assoc;
-    repeat rewrite Mscale_plus_distr_r with (x := ((-1)%R : C));
-    repeat rewrite Mplus_assoc.
-
-Definition error_decode_correct_no_error :
+Theorem error_decode_correct_no_error :
   forall (α β : C),
   (@uc_eval dim (apply_error NoError; decode)) × (encoded α β)
   = (α .* ∣0⟩ .+ β .* ∣1⟩) ⊗ ancillae_for NoError.
 Proof.
-  intros. subst.
-  Local Opaque decode CCX.
+  intros.
   simpl ancillae_for. Msimpl_light.
+  Local Opaque decode.
   simpl uc_eval. restore_dims.
-  repeat rewrite denote_SKIP; try lia.
-  repeat rewrite Mmult_1_l; auto 10 with wf_db.
-  restore_dims.
-  prep_err_compute.
   Local Transparent decode.
+  repeat rewrite denote_SKIP; try lia.
+  repeat rewrite Mmult_assoc; restore_dims.
+  repeat rewrite Mmult_1_l by auto 10 with wf_db.
+  rewrite decode_correct.
+  simpl (_ ⨂  _).
+  now rewrite kron_1_l by auto with wf_db.
+Qed.
 
-  assert (H1 :
-    (uc_eval decode
-          × f_to_vec (3 + 3 + 3)
-              (fun x : nat =>
-               if x <? 3 + 3
-               then if x <? 3 then false else false
-               else false))
-    = (/ C2 * / √ 2 )%C .* ((∣0,0,0⟩ .+ ∣1,0,0⟩) ⊗ (
-        ∣0, 0, 0, 0, 0, 0⟩
-     .+ ∣0, 0, 0, 1, 0, 0⟩
-     .+ ∣1, 0, 0, 0, 0, 0⟩
-     .+ ∣1, 0, 0, 1, 0, 0⟩))).
-  {
-    compute_vec.
-    post_compute_vec.
-    do 2 rewrite Mplus_comm with (A := ∣ 1, 0, 0, 1, 0, 0, 0, 0, 0 ⟩).
-    do 2 rewrite Mplus_comm with (A := ∣ 1, 0, 0, 1, 0, 0, 1, 0, 0 ⟩).
-    repeat rewrite Mplus_assoc.
-    do 2 rewrite Mplus_comm with (A := ∣ 1, 0, 0, 0, 0, 0, 1, 0, 0 ⟩).
-    repeat rewrite Mplus_assoc.
-    reflexivity.
-  }
-  rewrite H1. clear H1.
+Lemma Z_block_zero :
+  forall (off : block_offset), @uc_eval block_dim (SQIR.Z off) × ∣0,0,0⟩ = ∣0,0,0⟩.
+Proof.
+  intros.
+  destruct off; rewrite denote_Z; lma'.
+Qed.
 
-  assert (H2 :
-    (uc_eval decode
-              × f_to_vec (3 + 3 + 3)
-                  (fun x : nat =>
-                   if x <? 3 + 3
-                   then if x <? 3 then false else true
-                   else false))
-    = (
-      / C2 * / √ 2
-      .* (
-        (∣0, 0, 0⟩ ⊗ (∣0, 0, 0, 0, 0, 0⟩ .+ ∣0, 0, 0, 1, 0, 0⟩
-                    .+ ∣1, 0, 0, 1, 0, 0⟩ .+ (-1)%R .* ∣1, 0, 0, 0, 0, 0⟩))
-      .+ (∣1, 0, 0⟩ ⊗ ((-1)%R .* ∣1, 0, 0, 1, 0, 0⟩ .+           ∣1, 0, 0, 0, 0, 0⟩
-                   .+  (-1)%R .* ∣0, 0, 0, 1, 0, 0⟩ .+ (-1)%R .* ∣0, 0, 0, 0, 0, 0⟩))
-      )
-    )).
-  {
-    compute_vec.
-    replace ((-1)%R * / √ 2)%C with (/ √ 2 * (-1)%R)%C by apply Cmult_comm.
-    post_compute_vec.
+Lemma Z_block_seven :
+  forall (off : block_offset), @uc_eval block_dim (SQIR.Z off) × ∣1,1,1⟩ = (-1)%R .* ∣1,1,1⟩.
+Proof.
+  intros.
+  destruct off; rewrite denote_Z; lma'.
+Qed.
 
-    do 2 rewrite Mplus_comm with (A := ∣ 0, 0, 0, 1, 0, 0, 1, 0, 0 ⟩).
-    repeat rewrite Mplus_assoc.
-    reflexivity.
-  }
-  rewrite H2. clear H2.
+Definition post_one_phase_flip (α β : C) (n : block_no) :=
+  match n with
+  | Zer0 => (
+      α .* (/C2 .* (/√ 2 .* (
+          (∣0,0,0⟩ .+ (-1)%R .* ∣1,1,1⟩) ⊗ 2 ⨂ (∣0,0,0⟩ .+ ∣1,1,1⟩)))
+        )
+   .+ β .* (/C2 .* (/√ 2 .* (
+           (∣0,0,0⟩ .+ ∣1,1,1⟩) ⊗ 2 ⨂ (∣0,0,0⟩ .+ (-1)%R .* ∣1,1,1⟩)))
+        )
+  )
+  | One => (
+      α .* (/C2 .* (/√ 2 .* (
+          (∣0,0,0⟩ .+ ∣1,1,1⟩) ⊗ (∣0,0,0⟩ .+  (-1)%R .* ∣1,1,1⟩) ⊗ (∣0,0,0⟩ .+ ∣1,1,1⟩)))
+        )
+   .+ β .* (/C2 .* (/√ 2 .* (
+        (∣0,0,0⟩ .+ (-1)%R .* ∣1,1,1⟩) ⊗ (∣0,0,0⟩ .+ ∣1,1,1⟩) ⊗ (∣0,0,0⟩ .+ (-1)%R .* ∣1,1,1⟩)))
+        )
+  )
+  | Two => (
+      α .* (/C2 .* (/√ 2 .* (
+          (2 ⨂ (∣0,0,0⟩ .+ ∣1,1,1⟩) ⊗ (∣0,0,0⟩ .+ (-1)%R .* ∣1,1,1⟩)))
+        ))
+   .+ β .* (/C2 .* (/√ 2 .* (
+           2 ⨂ (∣0,0,0⟩ .+ (-1)%R .* ∣1,1,1⟩) ⊗ (∣0,0,0⟩ .+ ∣1,1,1⟩)))
+        )
+  )
+  end.
 
-  assert (H3 :
-    (uc_eval decode
-              × f_to_vec (3 + 3 + 3)
-                  (fun x : nat =>
-                   if x <? 3 + 3
-                   then if x <? 3 then true else false
-                   else false)) = 9 ⨂ ∣0⟩).
-  {
-    compute_vec.
-    repeat rewrite <- Cmult_assoc.
-    rewrite Cmult_comm with (x := ((-1)%R) : C).
-    post_compute_vec.
-    admit.
-  }
-  rewrite H3. clear H3.
+Theorem one_phase_flip_correct :
+  forall (α β : C) {n} (off : block_offset), 
+    uc_eval (apply_error (PhaseFlipError (OnePhaseFlip n off)))
+    × encoded α β 
+    = post_one_phase_flip α β n.
+Proof.
+  intros.
+  simpl uc_eval.
+  destruct n.
+  all : simpl (_ ⨂ _).
+  all : simpl apply_to_block.
+  all : simpl post_one_phase_flip.
+  all : correct_inPar ltac:(
+    (destruct off;
+      apply uc_well_typed_Z; simpl; lia)
+    || apply (@uc_well_typed_SKIP block_dim); lia
+  ).
+  all : distribute_over_blocks.
+  all : try rewrite denote_SKIP; try lia; Msimpl_light.
+  all : rewrite Z_block_zero, Z_block_seven.
+  all : repeat rewrite Mscale_assoc.
+  all : restore_dims.
+  all : replace ((-1)%R * (-1)%R)%C with C1 by lca.
+  all : now rewrite Mscale_1_l.
+Qed.
 
-  assert (H4 :
-    (uc_eval decode
-              × f_to_vec (3 + 3 + 3)
-                  (fun x : nat =>
-                   if x <? 3 + 3
-                   then if x <? 3 then true else true
-                   else false)) = 9 ⨂ ∣0⟩).
-  {
-    admit.
-  }
-  rewrite H4. clear H4.
+Theorem two_phase_flip_correct :
+  forall (α β : C) {n} (off₁ off₂ : block_offset), 
+    uc_eval (apply_error (PhaseFlipError (MorePhaseFlip n (OnePhaseFlip n off₁) off₂)))
+    × encoded α β 
+    = encoded α β.
+Proof.
+  intros.
+  simpl uc_eval.
+  destruct n.
+  all : simpl (_ ⨂ _).
+  all : simpl apply_to_block.
+  all : do 2 correct_inPar ltac:(
+    (destruct off₁; destruct off₂;
+      apply uc_well_typed_Z; simpl; lia)
+    || apply (@uc_well_typed_SKIP block_dim); lia
+  ).
+  all : distribute_over_blocks.
+  all : try rewrite denote_SKIP; try lia; Msimpl_light.
+  all : restore_dims.
+  all : repeat rewrite Mmult_assoc.
+  all : rewrite Z_block_zero, Z_block_seven.
+  all : repeat rewrite Mscale_mult_dist_r.
+  all : rewrite Z_block_zero, Z_block_seven.
+  all : repeat rewrite Mscale_assoc.
+  all : replace ((-1)%R * (-1)%R)%C with C1 by lca.
+  all : rewrite <- Mscale_assoc with (y := C1).
+  all : now rewrite Mscale_1_l.
+Qed.
 
-  assert (H5 :
-    (uc_eval decode
-              × f_to_vec (3 + 3 + 3)
-                  (fun x : nat =>
-                   if x <? 3 + 3
-                   then if x <? 3 then false else false
-                   else true)) = 9 ⨂ ∣0⟩).
-  {
-    admit.
-  }
-  rewrite H5. clear H5.
+Theorem more_than_two_phase_flip_correct :
+  forall (α β : C) {n} (off₁ off₂ : block_offset) (e : phase_flip_error n), 
+    uc_eval (apply_error (PhaseFlipError (MorePhaseFlip n (MorePhaseFlip n e off₂) off₁)))
+    × encoded α β 
+    = uc_eval (apply_error (PhaseFlipError e)) × encoded α β.
+Proof.
+  intros.
+  simpl uc_eval.
+  destruct n.
+  all : simpl (_ ⨂ _).
+  all : simpl apply_to_block.
+  all : do 2 correct_inPar ltac:(
+    (destruct off₁; destruct off₂;
+      apply uc_well_typed_Z; simpl; lia)
+    || apply (@uc_well_typed_SKIP block_dim); lia
+  ).
+  all : distribute_over_blocks.
+  all : try rewrite denote_SKIP; try lia; Msimpl_light.
+  all : restore_dims.
+  all : repeat rewrite Mmult_assoc.
+  all : rewrite Z_block_zero, Z_block_seven.
+  all : repeat rewrite Mscale_mult_dist_r.
+  all : rewrite Z_block_zero, Z_block_seven.
+  all : repeat rewrite Mscale_assoc.
+  all : replace ((-1)%R * (-1)%R)%C with C1 by lca.
+  all : rewrite <- Mscale_assoc with (y := C1).
+  all : now rewrite Mscale_1_l.
+Qed.
 
-  assert (H6 :
-    (uc_eval decode
-              × f_to_vec (3 + 3 + 3)
-                  (fun x : nat =>
-                   if x <? 3 + 3
-                   then if x <? 3 then false else true
-                   else true)) = 9 ⨂ ∣0⟩).
-  {
-    admit.
-  }
-  rewrite H6. clear H6.
+Lemma error_decode_correct_phase_flip_base :
+  forall (α β : C) {n} off,
+  (@uc_eval dim (apply_error (PhaseFlipError (OnePhaseFlip n off)); decode)) × (encoded α β)
+  = (α .* ∣0⟩ .+ β .* ∣1⟩) ⊗ ancillae_for (PhaseFlipError (OnePhaseFlip n off)).
+Proof.
+  intros.
+  Local Opaque apply_error.
+  simpl uc_eval.
+  rewrite Mmult_assoc.
+  rewrite one_phase_flip_correct.
+  destruct n.
+  all : simpl ancillae_for; simpl post_one_phase_flip.
+  par : now compute_decoding.
+Qed.
 
-  assert (H7 :
-    (uc_eval decode
-              × f_to_vec (3 + 3 + 3)
-                  (fun x : nat =>
-                   if x <? 3 + 3
-                   then if x <? 3 then true else false
-                   else true)) = 9 ⨂ ∣0⟩).
-  {
-    admit.
-  }
-  rewrite H7. clear H7.
+Theorem error_decode_correct_phase_flip :
+  forall (α β : C) {n} (e : @phase_flip_error n),
+  (@uc_eval dim (apply_error (PhaseFlipError e); decode)) × (encoded α β)
+  = (α .* ∣0⟩ .+ β .* ∣1⟩) ⊗ ancillae_for (PhaseFlipError e).
+Proof.
+  Local Opaque decode.
+  intros.
+  enough (
+    (@uc_eval dim (apply_error (PhaseFlipError e); decode)) × (encoded α β)
+      = (α .* ∣0⟩ .+ β .* ∣1⟩) ⊗ ancillae_for (PhaseFlipError e)
+    /\
+    forall off,
+    (@uc_eval dim (apply_error (PhaseFlipError (MorePhaseFlip n e off)); decode)) × (encoded α β)
+      = (α .* ∣0⟩ .+ β .* ∣1⟩) ⊗ ancillae_for (PhaseFlipError (MorePhaseFlip n e off))
+  ).
+  { destruct H; assumption. }
+  induction e.
+  - split.
+    + apply error_decode_correct_phase_flip_base.
+    + intros.
+      simpl uc_eval.
+      rewrite Mmult_assoc.
+      rewrite two_phase_flip_correct.
+      apply decode_correct.
+  - destruct IHe as [IHe IHme].
+    split.
+    + apply IHme.
+    + intros off0.
+      simpl uc_eval.
+      rewrite Mmult_assoc.
+      rewrite more_than_two_phase_flip_correct.
+      rewrite ancillae_for_two_phases_cancel.
+      simpl uc_eval in IHe.
+      rewrite Mmult_assoc in IHe.
+      apply IHe.
+Qed.
 
-  assert (H8 :
-    (uc_eval decode
-              × f_to_vec (3 + 3 + 3)
-                  (fun x : nat =>
-                   if x <? 3 + 3
-                   then if x <? 3 then true else true
-                   else true)) = 9 ⨂ ∣0⟩).
-  {
-    admit.
-  }
-  rewrite H8. clear H8.
 
-  restore_dims.
-  
-Admitted.
+Theorem error_decode_correct_bit_flip :
+  forall (α β : C) e,
+  (@uc_eval dim (apply_error (BitFlipError e); decode)) × (encoded α β)
+  = (α .* ∣0⟩ .+ β .* ∣1⟩) ⊗ ancillae_for (BitFlipError e).
+Proof.
+  intros.
+  Local Opaque decode_block.
+  destruct e.
+  all : repeat rewrite <- Mmult_assoc.
+  all : rewrite Mmult_plus_distr_l.
+  all : repeat rewrite Mscale_mult_dist_r.
+  2 : destruct safe_n.
+  1 : destruct n.
+  Local Transparent apply_error.
+  all : simpl uc_eval.
+  all : simpl (_ ⨂ _).
+  all : repeat rewrite Mmult_assoc; restore_dims.
+  all : simpl apply_to_block.
+  all : try rewrite kron_1_l by auto with wf_db.
+  all : restore_dims.
+  all : repeat rewrite kron_assoc by auto 10 with wf_db.
+  all : correct_inPar ltac:(
+    try apply decode_block_well_typed
+  ).
+  all : correct_inPar ltac:(
+    try apply uc_well_typed_X;
+    first [destruct off | destruct off₁; destruct off₂];
+    try destruct off₃; simpl; lia 
+    || apply (@uc_well_typed_SKIP block_dim); lia
+  ).
+  all : simpl (_ + _).
+  all : distribute_over_blocks.
+  all : try rewrite denote_SKIP; try lia; Msimpl_light.
+  all : first [destruct off | destruct off₁; destruct off₂];
+    try destruct off₃; simpl uc_eval; simpl ancillae_for.
+  (* slow; around ~2m *)
+  all : simpl apply_error.
+  par : restore_dims;
+  autorewrite with f_to_vec_3_db;
+  try repeat rewrite f_to_vec_X; try lia; simpl f_to_vec;
+  repeat rewrite kron_1_l by auto with wf_db;
+  restore_dims;
+  autorewrite with decode_block_db;
+  reorder_scalars; restore_dims;
+  repeat simplify_sums;
+  pull_scalars; restore_dims;
+  autorewrite with f_to_vec_3_db;
+  restore_dims;
+  repeat rewrite kron_assoc by auto 10 with wf_db;
+  repeat (rewrite f_to_vec_merge; restore_dims);
+  repeat Common.f_to_vec_simpl_light;
+  simpl f_to_vec; Msimpl_light;
+  repeat rewrite <- Cmult_assoc;
+  rewrite collapse_scalar; autorewrite with C_db;
+  now flatten.
+Qed.
 
 
 Definition shor_correct (e : error) : forall (α β : C),
@@ -532,7 +785,16 @@ Proof.
     simpl ancillae_for in H.
     rewrite Mmult_assoc in H.
     apply H.
-  - 
+  - simpl ancillae_for.
+    specialize (error_decode_correct_phase_flip α β e) as H.
+    simpl uc_eval in H.
+    rewrite Mmult_assoc in H.
+    apply H.
+  - simpl ancillae_for.
+    specialize (error_decode_correct_bit_flip α β e) as H.
+    simpl uc_eval in H.
+    rewrite Mmult_assoc in H.
+    apply H.
 Admitted.
 
 End NineQubitCode.
